adaptation to new outline

doc-src/Codegen/Thy/Refinement.thy
@@ -4,4 +4,109 @@ begin
 
 section {* Program and datatype refinement \label{sec:refinement} *}
 
+subsection {* Datatypes \label{sec:datatypes} *}
+
+text {*
+  Conceptually, any datatype is spanned by a set of
+  \emph{constructors} of type @{text "\<tau> = \<dots> \<Rightarrow> \<kappa> \<alpha>\<^isub>1 \<dots> \<alpha>\<^isub>n"} where @{text
+  "{\<alpha>\<^isub>1, \<dots>, \<alpha>\<^isub>n}"} is exactly the set of \emph{all} type variables in
+  @{text "\<tau>"}.  The HOL datatype package by default registers any new
+  datatype in the table of datatypes, which may be inspected using the
+  @{command print_codesetup} command.
+
+  In some cases, it is appropriate to alter or extend this table.  As
+  an example, we will develop an alternative representation of the
+  queue example given in \secref{sec:queue_example}.  The amortised
+  representation is convenient for generating code but exposes its
+  \qt{implementation} details, which may be cumbersome when proving
+  theorems about it.  Therefore, here is a simple, straightforward
+  representation of queues:
+*}
+
+datatype %quote 'a queue = Queue "'a list"
+
+definition %quote empty :: "'a queue" where
+  "empty = Queue []"
+
+primrec %quote enqueue :: "'a \<Rightarrow> 'a queue \<Rightarrow> 'a queue" where
+  "enqueue x (Queue xs) = Queue (xs @ [x])"
+
+fun %quote dequeue :: "'a queue \<Rightarrow> 'a option \<times> 'a queue" where
+    "dequeue (Queue []) = (None, Queue [])"
+  | "dequeue (Queue (x # xs)) = (Some x, Queue xs)"
+
+text {*
+  \noindent This we can use directly for proving;  for executing,
+  we provide an alternative characterisation:
+*}
+
+definition %quote AQueue :: "'a list \<Rightarrow> 'a list \<Rightarrow> 'a queue" where
+  "AQueue xs ys = Queue (ys @ rev xs)"
+
+code_datatype %quote AQueue
+
+text {*
+  \noindent Here we define a \qt{constructor} @{const "AQueue"} which
+  is defined in terms of @{text "Queue"} and interprets its arguments
+  according to what the \emph{content} of an amortised queue is supposed
+  to be.  Equipped with this, we are able to prove the following equations
+  for our primitive queue operations which \qt{implement} the simple
+  queues in an amortised fashion:
+*}
+
+lemma %quote empty_AQueue [code]:
+  "empty = AQueue [] []"
+  unfolding AQueue_def empty_def by simp
+
+lemma %quote enqueue_AQueue [code]:
+  "enqueue x (AQueue xs ys) = AQueue (x # xs) ys"
+  unfolding AQueue_def by simp
+
+lemma %quote dequeue_AQueue [code]:
+  "dequeue (AQueue xs []) =
+    (if xs = [] then (None, AQueue [] [])
+    else dequeue (AQueue [] (rev xs)))"
+  "dequeue (AQueue xs (y # ys)) = (Some y, AQueue xs ys)"
+  unfolding AQueue_def by simp_all
+
+text {*
+  \noindent For completeness, we provide a substitute for the
+  @{text case} combinator on queues:
+*}
+
+lemma %quote queue_case_AQueue [code]:
+  "queue_case f (AQueue xs ys) = f (ys @ rev xs)"
+  unfolding AQueue_def by simp
+
+text {*
+  \noindent The resulting code looks as expected:
+*}
+
+text %quote {*@{code_stmts empty enqueue dequeue (SML)}*}
+
+text {*
+  \noindent From this example, it can be glimpsed that using own
+  constructor sets is a little delicate since it changes the set of
+  valid patterns for values of that type.  Without going into much
+  detail, here some practical hints:
+
+  \begin{itemize}
+
+    \item When changing the constructor set for datatypes, take care
+      to provide alternative equations for the @{text case} combinator.
+
+    \item Values in the target language need not to be normalised --
+      different values in the target language may represent the same
+      value in the logic.
+
+    \item Usually, a good methodology to deal with the subtleties of
+      pattern matching is to see the type as an abstract type: provide
+      a set of operations which operate on the concrete representation
+      of the type, and derive further operations by combinations of
+      these primitive ones, without relying on a particular
+      representation.
+
+  \end{itemize}
+*}
+
 end
